Manually merge Negotiation.fst from quic2c

src/tls/Negotiation.fst
@@ -181,11 +181,6 @@ let find_signature_algorithms_cert o : option signatureSchemeList =
   | None -> None
   | Some (Extensions.E_signature_algorithms_cert algs) -> Some algs
 
-let find_quic_parameters o: option TLSConstants.quicParameters =
-  match find_client_extension Extensions.E_quic_parameters? o with
-  | Some (Extensions.E_quic_parameters qp) -> Some qp
-  | _ -> None
-
 let find_cookie o =
   match find_client_extension Extensions.E_cookie? o with
   | None -> None
@@ -319,11 +314,6 @@ let find_server_extension filter m =
   | None -> None
   | Some es -> List.Tot.find filter es
 
-let find_server_quic_parameters m =
-  match find_server_extension Extensions.E_quic_parameters? m with
-  | Some (Extensions.E_quic_parameters qp) -> Some qp
-  | _ -> None
-
 let is_resumption12 m =
   not (is_pv_13 m.n_protocol_version)  &&
   m.n_sessionID = m.n_offer.ch_sessionID
@@ -418,9 +408,9 @@ noeq type t (region:rgn) (role:TLSConstants.role) : Type0 =
 
 #set-options "--lax"
 val computeOffer: r:role -> cfg:config -> resume:TLSInfo.resumeInfo r -> nonce:TLSInfo.random
-  -> ks:option CommonDH.keyShare -> list (PSK.pskid * PSK.pskInfo)
+  -> ks:option CommonDH.keyShare -> list (PSK.pskid * PSK.pskInfo) -> UInt32.t
   -> Tot offer
-let computeOffer r cfg resume nonce ks pskinfo =
+let computeOffer r cfg resume nonce ks pskinfo now =
   let ticket12, sid =
     match resume, cfg.enable_tickets, cfg.min_version with
     | _, _, TLS_1p3 -> None, empty_bytes // Don't bother sending session_ticket
@@ -438,10 +428,6 @@ let computeOffer r cfg resume nonce ks pskinfo =
     match pskinfo with
     | (_, i) :: _ -> i.allow_early_data // Must be the first PSK
     | _ -> false in
-  let qp =
-    match cfg.quic_parameters with
-    | Some (qv::_, qp) -> Some (QuicParametersClient qv qp)
-    | _ -> None in
   let extensions =
     Extensions.prepareExtensions
       cfg.min_version
@@ -449,7 +435,8 @@ let computeOffer r cfg resume nonce ks pskinfo =
       cfg.cipher_suites
       cfg.peer_name
       cfg.alpn
-      qp
+      cfg.custom_extensions
+      // qp
       cfg.extended_master_secret
       cfg.safe_renegotiation
       (compatible_psk && Some? cfg.max_early_data)
@@ -459,6 +446,7 @@ let computeOffer r cfg resume nonce ks pskinfo =
       None // : option (cVerifyData * sVerifyData)
       ks
       pskinfo
+      now
   in
   {
     ch_protocol_version = minPV TLS_1p2 cfg.max_version; // legacy for 1.3
@@ -646,40 +634,30 @@ let rec map_ST f x = match x with
 
 let i_psk_info i = (i, PSK.psk_info i)
 
-// cwinter: unused?
-// val client_ClientHello: #region:rgn -> t region Client
-//   -> option CommonDH.clientKeyShare
-//   -> St offer
-//   // requires C_Init? i.e.  st = transcript_state client_config []
-//   // ensures C_offer? i.e. st = transcript_state client_config [ClientHello offer]
-//   //                                /\ witnessed (fun h -> sel h st == offer)
-
-//   (ensures fun h0 offer h1 ->
-//     let st0 = sel h0 n in
-//     let st1 = sel h1 n in
-//     offer_v st == offer /\ (* also use computeOffer here? *)
-//     replay_transcript st0.config [ClientHello offer] (*ghost*) == Correct st1)
-
-// let client_ClientHello #region ns oks =
-//   //17-04-22 fix this in the definition of offer?
-//   let oks' =
-//     match oks with
-//     | Some ks -> Some (CommonDH.ClientKeyShare ks)
-//     | None -> None in
-//   let _, pskid = ns.resume in
-//   let pskinfo = map_ST i_psk_info pskid in
-//   match HST.op_Bang ns.state with
-//   | C_Init _ ->
-//       trace(if
-//         (match pskinfo with
-//         | (_, i) :: _ -> i.allow_early_data && Some? ns.cfg.max_early_data // Must be the first PSK
-//         | _ -> false)
-//       then "Offering a PSK compatible with 0-RTT" else "No PSK or 0-RTT disabled");
-//       let offer = computeOffer Client ns.cfg ns.resume ns.nonce oks' pskinfo in
-//       trace ("offering client extensions "^string_of_option_extensions offer.ch_extensions);
-//       trace ("offering cipher suites "^string_of_ciphersuites offer.ch_cipher_suites);
-//       HST.op_Colon_Equals ns.state (C_Offer offer);
-//       offer
+val client_ClientHello: #region:rgn -> t region Client
+  -> option CommonDH.clientKeyShare
+  -> St offer
+let client_ClientHello #region ns oks =
+  //17-04-22 fix this in the definition of offer?
+  let oks' =
+    match oks with
+    | Some ks -> Some (CommonDH.ClientKeyShare ks)
+    | None -> None in
+  let _, pskid = ns.resume in
+  let pskinfo = map_ST i_psk_info pskid in
+  match HST.op_Bang ns.state with
+  | C_Init _ ->
+      trace(if
+        (match pskinfo with
+        | (_, i) :: _ -> i.allow_early_data && Some? ns.cfg.max_early_data // Must be the first PSK
+        | _ -> false)
+      then "Offering a PSK compatible with 0-RTT" else "No PSK or 0-RTT disabled");
+      let now = CoreCrypto.now () in
+      let offer = computeOffer Client ns.cfg ns.resume ns.nonce oks' pskinfo now in
+      trace ("offering client extensions "^string_of_option_extensions offer.ch_extensions);
+      trace ("offering cipher suites "^string_of_ciphersuites offer.ch_cipher_suites);
+      HST.op_Colon_Equals ns.state (C_Offer offer);
+      offer
 
 let group_of_hrr hrr : option CommonDH.group =
   match List.Tot.find (Extensions.E_key_share?) hrr.hrr_extensions with
@@ -712,52 +690,27 @@ let client_HelloRetryRequest #region (ns:t region Client) hrr (s:option share) =
       match find_pske offer with
       | None -> []
       | Some pskl -> pskl in
-    let Some (| g, gx |) = s in
+    // TODO early data not recorded in retryInfo
+    let ext' = TLSConstants.choose_aux s choose_extension (Some?.v offer.ch_extensions) in
 
-    (match group_of_hrr hrr, find_supported_groups offer with
-    | Some g', Some ngl ->
-      if g = g' && List.Tot.mem (Some?.v (CommonDH.namedGroup_of_group g')) ngl then
-       begin
-        // TODO early data not recorded in retryInfo
-        let ext' = List.Tot.choose (fun (e:Extensions.extension) ->
-          if Extensions.E_key_share? e then
-            Some (Extensions.E_key_share
-             (CommonDH.ClientKeyShare [CommonDH.Share g gx]))
-          else if Extensions.E_early_data? e then None
-          else Some e // TODO filter PSK
-          ) (Some?.v offer.ch_extensions) in
+    // Echo the cookie for QUIC stateless retry
+    let ext', no_cookie = match List.Tot.find Extensions.E_cookie? el with
+      | Some cookie -> cookie :: ext', false
+      | None -> ext', true in
 
-        let offer' = {offer with ch_extensions = Some ext'} in
-        let ri = (hrr, old_shares, old_psk) in
-        ns.state := C_HRR offer' ri;
-        Correct(offer')
-       end
-      else
-        Error(AD_illegal_parameter, "server asked for an invalid group in HRR")
-    | _ ->
-      Error(AD_illegal_parameter, "only keyShare-based HRR is supported on client"))
-
-    // cwinter: quic2c
-    // // TODO early data not recorded in retryInfo
-    // let ext' = TLSConstants.choose_aux s choose_extension (Some?.v offer.ch_extensions) in
-
-    // // Echo the cookie for QUIC stateless retry
-    // let ext' = match List.Tot.find Extensions.E_cookie? el with
-    //   | Some cookie -> cookie :: ext'
-    //   | None -> ext' in
-
-    // if sid <> offer.ch_sessionID then
-    //   Error(AD_illegal_parameter, "mismatched session ID in HelloRetryRequest")
-    // else if None? (group_of_hrr hrr) && None? ns.cfg.quic_parameters then
-    //   Error(AD_illegal_parameter, "only keyShare-based HRR is supported on client")
-    // else
-    //  begin
-    //   let offer' = {offer with ch_extensions = Some ext'} in
-    //   let ri = (hrr, old_shares, old_psk) in
-    //   ns.state := (C_HRR offer' ri);
-    //   Correct(offer')
-    //  end
-
+    if sid <> offer.ch_sessionID then
+      Error(AD_illegal_parameter, "mismatched session ID in HelloRetryRequest")
+    // 2018.03.08 SZ: TODO We must Update PSK extension if present
+    // See https://tools.ietf.org/html/draft-ietf-tls-tls13-26#section-4.1.2
+    else if None? (group_of_hrr hrr) && no_cookie then
+      Error(AD_illegal_parameter, "received a HRR that would yield the same ClientHello")
+    else
+     begin
+      let offer' = {offer with ch_extensions = Some ext'} in
+      let ri = (hrr, old_shares, old_psk) in
+      ns.state := (C_HRR offer' ri);
+      Correct(offer')
+     end
 
 (**
   Checks that the protocol version in ClientHello is
@@ -1116,42 +1069,50 @@ let clientComplete_13 #region ns ee optCertRequest optServerCert optCertVerify d
       | None, [] -> None
       | None, ee -> Some ee
       in
-    let validSig, schain =
-      match kexAlg mode, optServerCert, optCertVerify, digest with
-      | Kex_DHE, Some c, Some cv, Some digest
-      | Kex_ECDHE, Some c, Some cv, Some digest ->
-        // TODO ensure that valid_offer mandates signature extensions for 1.3
-        let Some sal = find_signature_algorithms mode.n_offer in
-        let sa = Some?.v cv.sig_algorithm in
-        let chain = Some (c, sa) in
-        if List.Tot.mem sa sal then
-          let tbs = to_be_signed mode.n_protocol_version Server None digest in
-          cert_verify_cb ns.cfg (Cert.chain_down c) sa tbs cv.sig_signature, chain
-        else false, None // The server signed with an algorithm we did not offer
-      | Kex_PSK_ECDHE, None, None, None
-      | Kex_PSK, None, None, None -> true, None // FIXME recall chain from PSK
-      | _ -> false, None
-      in
-    trace ("Certificate & signature 1.3 callback result: " ^ (if validSig then "valid" else "invalid"));
-    if validSig then
-      let mode = Mode
-        mode.n_offer
-        mode.n_hrr
-        mode.n_protocol_version
-        mode.n_server_random
-        mode.n_sessionID
-        mode.n_cipher_suite
-        mode.n_pski
-        sexts
-        mode.n_server_share
-        optCertRequest
-        schain
-        mode.n_client_share
-      in
-      HST.op_Colon_Equals ns.state (C_Complete mode ccert);
-      Correct mode
-    else
-      Error(AD_bad_certificate_fatal, "Failed to validate signature or certificate")
+    let nego_cb = ns.cfg.nego_callback in
+    let exts = Extensions.app_ext_filter sexts in
+    let exts_bytes = HandshakeMessages.optionExtensionsBytes exts in
+    trace ("Negotiation callback to process application extensions.");
+    match nego_cb.negotiate nego_cb.nego_context mode.n_protocol_version exts_bytes None with
+    | Nego_abort -> Error(AD_handshake_failure, perror __SOURCE_FILE__ __LINE__ "application requested to abort the handshake")
+    | Nego_retry _ -> Error(AD_internal_error, perror __SOURCE_FILE__ __LINE__ "client application requested a server retry")
+    | Nego_accept _ ->
+      let validSig, schain =
+        match kexAlg mode, optServerCert, optCertVerify, digest with
+        | Kex_DHE, Some c, Some cv, Some digest
+        | Kex_ECDHE, Some c, Some cv, Some digest ->
+          // TODO ensure that valid_offer mandates signature extensions for 1.3
+          let Some sal = find_signature_algorithms mode.n_offer in
+          let sa = Some?.v cv.sig_algorithm in
+          let chain = Some (c, sa) in
+          if List.Tot.mem sa sal then
+            let tbs = to_be_signed mode.n_protocol_version Server None digest in
+            cert_verify_cb ns.cfg (Cert.chain_down c) sa tbs cv.sig_signature, chain
+          else false, None // The server signed with an algorithm we did not offer
+        | Kex_PSK_ECDHE, None, None, None
+        | Kex_PSK, None, None, None -> true, None // FIXME recall chain from PSK
+        | _ -> false, None
+        in
+      trace ("Certificate & signature 1.3 callback result: " ^ (if validSig then "valid" else "invalid"));
+      if validSig then
+        let mode = Mode
+          mode.n_offer
+          mode.n_hrr
+          mode.n_protocol_version
+          mode.n_server_random
+          mode.n_sessionID
+          mode.n_cipher_suite
+          mode.n_pski
+          sexts
+          mode.n_server_share
+          optCertRequest
+          schain
+          mode.n_client_share
+        in
+        HST.op_Colon_Equals ns.state (C_Complete mode ccert);
+        Correct mode
+      else
+        Error(AD_bad_certificate_fatal, "Failed to validate signature or certificate")
 
 (* SERVER *)
 
@@ -1271,10 +1232,15 @@ let rec register_shares (l:list pre_share)
   | [] -> []
   | (| g, gx |) :: t -> (| g, CommonDH.register_dhi #g gx |) :: (register_shares t)
 
+// For application-handled extensions set by nego callback,
+// such as QUIC transport parameters
+type extra_ext = // list (e:Extensions.extension{E_unknown_extension? e})
+  list Extensions.extension
+
 //17-03-30 still missing a few for servers.
 type serverMode =
   | ServerHelloRetryRequest: hrr -> serverMode
-  | ServerMode: mode -> certNego -> serverMode
+  | ServerMode: mode -> certNego -> extra_ext -> serverMode
 
 let get_sni (o:offer) : bytes =
   match find_client_extension Extensions.E_server_name? o with
@@ -1304,7 +1270,8 @@ let computeServerMode cfg co serverRandom =
           List.Helpers.filter_aux cfg.signature_algorithms List.Helpers.mem_rev sigalgs
         in
         if sigalgs = [] then None
-        else cert_select_cb cfg (get_sni co) sigalgs
+        // FIXME(adl) workaround for a bug in TLSConstants that causes signature schemes list to be parsed in reverse order
+        else cert_select_cb cfg (get_sni co) (List.Tot.rev sigalgs)
       in
     match compute_cs13 cfg co pske shares (Some? scert) with
     | Error z -> Error z
@@ -1316,7 +1283,6 @@ let computeServerMode cfg co serverRandom =
         hrr_extensions = [
           Extensions.E_supported_versions (Extensions.ServerPV TLS_1p3);
           Extensions.E_key_share (CommonDH.HRRKeyShare ng);
-          Extensions.E_cookie (CoreCrypto.random 32)
         ]; } in
       Correct(ServerHelloRetryRequest hrr)
     | Correct ((PSK_EDH j ogx cs)::_, _) ->
@@ -1334,7 +1300,7 @@ let computeServerMode cfg co serverRandom =
         None // TODO: n_client_cert_request
         None
         ogx)
-      None)) // No cert
+      None [])) // No cert
     | Correct ((JUST_EDH gx cs) :: _, _) ->
       (trace "Negotiated Pure EDH key exchange";
       let Some (cert, sa) = scert in
@@ -1355,7 +1321,7 @@ let computeServerMode cfg co serverRandom =
           None // TODO: n_client_cert_request
           (Some (Cert.chain_up schain, sa))
           (Some gx))
-        scert))
+        scert []))
     end
   | Correct pv ->
     let valid_ticket =
@@ -1380,7 +1346,7 @@ let computeServerMode cfg co serverRandom =
         None
         None
         None
-        None) None)
+        None) None [])
     | _ ->
       // Make sure NullCompression is offered
       if not (List.Tot.mem NullCompression co.ch_compressions)
@@ -1413,7 +1379,7 @@ let computeServerMode cfg co serverRandom =
                 None
                 (Some (Cert.chain_up schain, sa))
                 None) // no client key share yet for 1.2
-              (Some(cert, sa))
+              (Some(cert, sa)) []
             ))
 
 private
@@ -1451,9 +1417,9 @@ let rec forall_aux (#a:Type) (#b:Type) (env:b) (f: b -> a -> Tot bool) (l:list a
     | hd::tl -> if f env hd then forall_aux env f tl else false
             
 val server_ClientHello: #region:rgn -> t region Server ->
-  HandshakeMessages.ch ->
+  HandshakeMessages.ch -> log:HandshakeLog.t ->
   St (result serverMode)
-let server_ClientHello #region ns offer =
+let server_ClientHello #region ns offer log =
   trace ("offered client extensions "^string_of_option_extensions offer.ch_extensions);
   trace ("offered cipher suites "^(string_of_ciphersuites offer.ch_cipher_suites));
   trace (match (offered_versions TLS_1p0 offer) with
@@ -1461,6 +1427,7 @@ let server_ClientHello #region ns offer =
         | Correct v -> List.Tot.fold_left accum_string_of_pv "offered versions" v);
   match HST.op_Bang ns.state with
   | S_HRR o1 hrr ->
+    trace ("Processing second offer based on existing HRR state (staeful HRR).");
     let o2 = offer in
     if
       o1.ch_protocol_version = o2.ch_protocol_version &&
@@ -1479,52 +1446,94 @@ let server_ClientHello #region ns offer =
         Error z
       | Correct (ServerHelloRetryRequest hrr) ->
         Error(AD_illegal_parameter, "client sent the same hello in response to hello retry")
-      | Correct(ServerMode m cert) ->
+      | Correct (ServerMode m cert _) ->
         trace ("negotiated after HRR "^string_of_pv m.n_protocol_version^" "^string_of_ciphersuite m.n_cipher_suite);
-        HST.op_Colon_Equals ns.state (S_ClientHello m cert);
-        sm
+        let nego_cb = ns.cfg.nego_callback in
+        let exts = Extensions.app_ext_filter offer.ch_extensions in
+        let exts_bytes = HandshakeMessages.optionExtensionsBytes exts in
+        trace ("Negotiation callback to handle extra extensions.");
+        match nego_cb.negotiate nego_cb.nego_context m.n_protocol_version exts_bytes (Some empty_bytes) with
+        | Nego_accept sexts ->
+          let el = Extensions.ext_of_custom sexts in
+          HST.op_Colon_Equals ns.state (S_ClientHello m cert);
+          Correct (ServerMode m cert el)
+        | _ ->
+          trace ("Application requested to abort the handshake after internal HRR.");
+          Error (AD_handshake_failure, "application aborted the handshake by callback")
     else
       Error(AD_illegal_parameter, "Inconsistant parameters between first and second client hello")
   | S_Init _ ->
     let sm = computeServerMode ns.cfg offer ns.nonce in
+    let previous_cookie = // for stateless HRR
+      match find_cookie offer with
+      | None -> None
+      | Some c ->
+        match Ticket.check_cookie c with
+        | None -> trace ("WARNING: ignorning invalid cookie "^(hex_of_bytes c)); None
+        | Some (hrr, digest, extra) ->
+          trace ("Loaded stateless retry cookie "^(hex_of_bytes c));
+          let hrr = { hrr with hrr_extensions =
+            (Extensions.E_cookie c) :: hrr.hrr_extensions; } in
+          // Overwrite the current transcript digest with values from cookie
+          trace ("Overwriting the transcript digest with CH1 hash "^(hex_of_bytes digest));
+          HandshakeLog.load_stateless_cookie log hrr digest;
+          Some extra // for the server nego callback
+      in
     match sm with
     | Error z ->
       trace ("negotiation failed: "^string_of_error z);
       Error z
     | Correct (ServerHelloRetryRequest hrr) ->
+      // Internal HRR caused by group negotiation
+      // We do not invoke the server nego callback in this case
       // record the initial offer and return the HRR to HS
       ns.state := S_HRR offer hrr;
       sm
     | Correct (ServerMode m certNego) ->
       trace ("negotiated "^string_of_pv m.n_protocol_version^" "^string_of_ciphersuite m.n_cipher_suite);      
-      // cwinter: does this belong here?
-      // ns.state := S_HRR offer hrr;
+      let ha = verifyDataHashAlg_of_ciphersuite hrr.hrr_cipher_suite in
+      let digest = HandshakeLog.hash_tag #ha log in
+      let cookie = Ticket.create_cookie hrr digest empty_bytes in
+      let hrr = { hrr with hrr_extensions =
+        (Extensions.E_cookie cookie) :: hrr.hrr_extensions; } in
+      HST.op_Colon_Equals ns.state (S_HRR offer hrr);
       sm
-    | Correct (ServerMode m cert) ->
-      // Forcing HRR for source address validation
-      if ns.cfg.offer_shares = [] then
+    | Correct (ServerMode m cert _) ->
+      let nego_cb = ns.cfg.nego_callback in
+      let exts = Extensions.app_ext_filter offer.ch_extensions in
+      let exts_bytes = HandshakeMessages.optionExtensionsBytes exts in
+      trace ("Negotiation callback to handle extra extensions and query for stateless retry.");
+      trace ("Application data in cookie: "^(match previous_cookie with | Some c -> hex_of_bytes c | _ -> "none"));
+      match nego_cb.negotiate nego_cb.nego_context m.n_protocol_version exts_bytes previous_cookie with
+      | Nego_abort ->
+        trace ("Application requested to abort the handshake.");
+        Error (AD_handshake_failure, "application aborted the handshake by callback")
+      | Nego_retry cextra ->
         let hrr = ({
           hrr_sessionID = offer.ch_sessionID;
           hrr_cipher_suite = m.n_cipher_suite;
           hrr_extensions = [
             Extensions.E_supported_versions (Extensions.ServerPV TLS_1p3);
-            Extensions.E_cookie (CoreCrypto.random 32)
           ]}) in
-        ns.state := S_HRR offer hrr;
+        let ha = verifyDataHashAlg_of_ciphersuite hrr.hrr_cipher_suite in
+        let digest = HandshakeLog.hash_tag #ha log in
+        let cookie = Ticket.create_cookie hrr digest cextra in
+        let hrr = { hrr with hrr_extensions =
+          (Extensions.E_cookie cookie) :: hrr.hrr_extensions; } in
+        ns.state := (S_HRR offer hrr);
         Correct (ServerHelloRetryRequest hrr)
-      else
-       begin
+      | Nego_accept sexts ->
         trace ("negotiated "^string_of_pv m.n_protocol_version^" "^string_of_ciphersuite m.n_cipher_suite);
-        ns.state := (S_ClientHello m cert);
-        sm
-       end
+        ns.state := S_ClientHello m cert;
+        Correct (ServerMode m cert (Extensions.ext_of_custom sexts))
 
 let share_of_serverKeyShare (ks:CommonDH.serverKeyShare) : share =
   let CommonDH.Share g gy = ks in (| g, gy |)
 
-val server_ServerShare: #region:rgn -> t region Server -> option CommonDH.serverKeyShare  ->
+val server_ServerShare: #region:rgn -> t region Server ->
+  option CommonDH.serverKeyShare -> extra_ext ->
   St (result mode)
-let server_ServerShare #region ns ks =
+let server_ServerShare #region ns ks app_exts =
   match HST.op_Bang ns.state with
   | S_ClientHello mode cert ->
     let cexts = mode.n_offer.ch_extensions in
@@ -1544,6 +1553,12 @@ let server_ServerShare #region ns ks =
     | Correct sexts ->
       begin
       trace ("including server extensions (SH + EE) " ^ string_of_option_extensions sexts);
+      let sexts = match sexts with
+        | Some el ->
+          trace ("extra extensions from application callback: "^string_of_extensions app_exts);
+          Some (el @ app_exts)
+        | _ -> sexts
+        in
       let mode = Mode
         mode.n_offer
         mode.n_hrr
